Source/DafnyCore/Verifier/Statements/OpaqueBlockVerifier.cs
@@ -1,4 +1,5 @@
 using System.Collections.Generic;
+using System.Diagnostics.Contracts;
 using System.Linq;
 using Microsoft.Boogie;
 using DafnyIdentifierExpr = Microsoft.Dafny.IdentifierExpr;
@@ -60,7 +61,15 @@ public static class OpaqueBlockVerifier {
         new TypedIdent(block.Origin, uniqueId, generator.Predef.HeapType)));
       builder.Add(Cmd.SimpleAssign(block.Origin, new Boogie.IdentifierExpr(block.Origin, heapAtVariable), etran.HeapExpr));
 
-      beforeBlockExpressionTranslator = etran.WithHeapVariable(uniqueId);
+      beforeBlockExpressionTranslator = etran.WithHeapVariable(uniqueId, out var uniqueIdReferrers);
+
+      if (builder.Options.Get(CommonOptionBag.Referrers)) {
+        Contract.Assert(uniqueIdReferrers != null);
+        var referrersHeapAtVariable = locals.GetOrAdd(new Boogie.LocalVariable(block.Origin,
+          new TypedIdent(block.Origin, uniqueIdReferrers, generator.Predef.ReferrersHeapType)));
+        builder.Add(Cmd.SimpleAssign(block.Origin, new BoogieIdentifierExpr(block.Origin, referrersHeapAtVariable),
+          etran.ReferrersHeapExpr));
+      }
     } else {
       beforeBlockExpressionTranslator = etran;
     }
