Source/IntegrationTests/TestFiles/LitTests/LitTest/referrers/referrers-errors.dfy
@@ -1,0 +1,27 @@
+// RUN: %exits-with 4 %verify --referrers --type-system-refresh "%s" > "%t"
+// RUN: %diff "%s.expect" "%t"
+
+class Test {
+  var x: Test?
+  var y: Test?
+  const z: Test? := null;
+}
+
+method MethodMightNotRestoreReferrers() {
+  var t = new Test();
+  assert referrers(t) == {locals`t};
+  CallSubMethod(t);
+  assert referrers(t) == {locals`t}; // Error: Cannot prove this
+}
+
+// No referrers clause means we don't know what happens to any object.
+method CallSubMethod(t: Test)
+{
+}
+
+method EnsuresReferrersUnchanged(t2: Test)
+  ensures old(referrers(t2)) == referrers(t2)
+{
+  var t_local := t2;
+  assert referrers(t_local) == old(referrers(t_local)) + {locals`t_local}; // Error, t_local was not assigned
+}
