Source/IntegrationTests/TestFiles/LitTests/LitTest/referrers/referrers-resolutionerrors.dfy
@@ -1,0 +1,15 @@
+// RUN: %exits-with 2 %resolve --referrers --type-system-refresh "%s" > "%t"
+// RUN: %diff "%s.expect" "%t"
+
+class Test {
+  var x: Test?
+  var y: Test?
+  const z: Test? := null;
+}
+
+datatype X = X()
+
+method Test() {
+  assert referrers(X()) == {}; // Error, referrers should be applied to a single object or array, got X
+  assert referrers(1) == {}; // Error, referrers should be applied to a single object or array, got int
+}
