Source/IntegrationTests/TestFiles/LitTests/LitTest/referrers/referrers.dfy
@@ -1,0 +1,148 @@
+// RUN: %verify --referrers --type-system-refresh "%s" > "%t"
+// RUN: %diff "%s.expect" "%t"
+
+
+class SimpleObject {
+}
+
+///// Local fields and input parameters
+
+method ReferrersLocal() {
+  var t := new SimpleObject;
+  assert referrers(t) == {locals`t};
+  var alias_t := t;
+  assert referrers(t) == {locals`t, locals`alias_t};
+  label before_t_null:
+  t := null;
+  assert referrers(alias_t) == {locals`alias_t};
+  assert old@before_t_null(referrers(alias_t#0)) == {locals`t, locals`alias_t};
+  
+  // Arrays too have referrers
+  var u := new SimpleObject?[1](i => null);
+  assert referrers(u) == {locals`u};
+}
+
+method ReferrersMethodCall(t: SimpleObject)
+{
+  assert locals`t in referrers(t);
+}
+
+// Input parameters are not unassigned when the method exits.
+// However, local variables in scope are unassigned before a return
+method EnsuresReferrersUnchanged(t2: SimpleObject)
+  ensures old(referrers(t2)) == referrers(t2)
+{
+  var t_local := t2;
+  assert old(referrers(t2)) == old(referrers(t_local)); // Local variables don't depend on any heap so they can be used in old expressions
+  assert referrers(t2) == old(referrers(t2)) + {locals`t_local};
+  return; // Here t_local is unassigned.
+}
+
+method CallReferrersMethodCall() {
+  var t := new SimpleObject;
+  assert referrers(t) == {locals`t};
+  EnsuresReferrersUnchanged(t); // Here t2 is added to the referrers, then the referrers are assumed to not be changed, and t2 is unassigned.
+  assert referrers(t) == {locals`t};
+}
+
+//// Ghost versions are the same //////
+
+ghost method GhostReferrersLocals() {
+  ghost var t := new SimpleObject;
+  assert referrers(t) == {locals`t};
+  ghost var alias_untracked := t;    // Even in ghost context, ghost markers means non-tracking by default.
+  assert referrers(t) == {locals`t};
+  ghost var {:tracking} alias_tracked := t; // This is not useful in practice in ghost methods since one can just declare normal variables, but it's here for coherence
+  assert referrers(t) == {locals`t, locals`alias_tracked};
+  
+  assert (locals`t.1).IsGhost;
+  assert (locals`alias_untracked.1).IsGhost;
+  assert (locals`alias_tracked.1).IsGhost;
+}
+
+method ReferrersLocalWithGhostAliases() {
+  var t := new SimpleObject;
+  assert referrers(t) == {locals`t};
+  ghost var alias_untracked := t;    // Ghost variables, like ghost fields, are non-tracking by default.
+  assert referrers(t) == {locals`t};
+  ghost var {:tracking} alias_tracked := t; // To make a ghost variable tracking, one must force it.
+  assert referrers(t) == {locals`t, locals`alias_tracked};
+  
+  assert !(locals`t.1).IsGhost;
+  assert (locals`alias_untracked.1).IsGhost;
+  assert (locals`alias_tracked.1).IsGhost;
+}
+
+
+method ReferrersOnGhostConstructedInstanceInCompiledContext() {
+  ghost var t := new SimpleObject; // Automatically marked as tracking when the RHS
+  assert referrers(t) == {};
+  ghost var alias_untracked := t;    // Ghost variables, like ghost fields, are non-tracking by default.
+  assert referrers(t) == {};
+  ghost var {:tracking} alias_tracked := t; // To make a ghost variable tracking, one must force it.
+  assert referrers(t) == {locals`alias_tracked};
+  
+  assert (locals`t.1).IsGhost;
+  assert (locals`alias_untracked.1).IsGhost;
+  assert (locals`alias_tracked.1).IsGhost;
+}
+
+
+///// Object fields and object constants
+
+class ChainingObject {
+  var x: ChainingObject?
+  var y: ChainingObject?
+  ghost var nontracking: ChainingObject?
+  ghost var {:tracking} tracking: ChainingObject?
+  const tail: ChainingObject?
+  constructor(chained_test: ChainingObject?) ensures x == y == nontracking == tracking == null && tail == chained_test
+    ensures chained_test != null ==> referrers(chained_test) == old(referrers(chained_test)) + {this`tail}
+    ensures forall o: object | o != chained_test :: referrers(o) == old(referrers(o)) // Replace by referrers clauses when they arrive
+  {
+    x := null;
+    y := null;
+    tracking := null;
+    nontracking := null;
+    tail := chained_test;
+  }
+}
+
+// Ghost parameters are untracking by default
+lemma CouldFree(t: object)
+  requires |set r: (object, field) <- referrers(t) | !r.1.IsGhost| == 1
+
+method ObjectFields() {
+  var t := new ChainingObject(null);
+  assert referrers(t) == {locals`t};
+  t.x := t;
+  assert referrers(t) == {locals`t, t`x};
+  t.y := t;
+  assert referrers(t) == {locals`t, t`x, t`y};
+  t.x := null;
+  assert referrers(t) == {locals`t, t`y};
+  t.y := null;
+  assert referrers(t) == {locals`t};
+  t.tracking := t; // Ghost assignment
+  assert referrers(t) == {locals`t, t`tracking};
+  t.tracking := null;
+  assert referrers(t) == {locals`t};
+  t.nontracking := t;
+  assert referrers(t) == {locals`t};  
+  CouldFree(t);
+  
+  var u := new ChainingObject(t);
+  assert referrers(u) == {locals`u};
+  assert referrers(t) == {locals`t, u`tail};
+  u.x := t;
+  assert referrers(t) == {locals`t, u`tail, u`x};
+  assert referrers(u) == {locals`u};
+  u.x := u; // Double change
+  assert referrers(t) == {locals`t, u`tail};
+  assert referrers(u) == {locals`u, u`x};
+  
+  // Assignment of array
+  var a := new ChainingObject[2](i => if i == 0 then t else u);
+  assert referrers(t) == {locals`t, u`tail, a`[0]};
+  assert referrers(u) == {locals`t, u`x, a`[1]};
+}
